Use a structure for Preserved relation

Clear/EVMState.lean
@@ -164,59 +164,50 @@ instance : Inhabited EVMState :=
 
 abbrev EVM := EVMState
 
-instance instFinmapPreorder : Preorder (Finmap (λ _ : List UInt256 ↦ UInt256)) where
+instance instPreorderFinmap : Preorder (Finmap (λ _ : List UInt256 ↦ UInt256)) where
   le a b := a.keys ⊆ b.keys ∧ ∀ {key}, key ∈ a → a.lookup key = b.lookup key
   le_refl := by aesop
   le_trans := by aesop (add safe forward subset_trans)
 
-def preserved : EVMState → EVMState → Prop :=
-  λ a b ↦ (Eq on EVMState.account_map) a b ∧
-          (Eq on EVMState.hash_collision) a b ∧
-          (Eq on EVMState.execution_env) a b ∧
-          (a.keccak_map ≤ b.keccak_map)
+structure Preserved (a : EVMState) (b : EVMState) : Prop where
+  account_map : (Eq on EVMState.account_map) a b
+  hash_collision : (Eq on EVMState.hash_collision) a b
+  execution_env : (Eq on EVMState.execution_env) a b
+  keccak_map : a.keccak_map ≤ b.keccak_map
 
-lemma preserved_def {σ₀ σ₁ : EVM} : preserved σ₀ σ₁ =
+lemma Preserved_def {σ₀ σ₁ : EVM} : Preserved σ₀ σ₁ =
   (σ₀.account_map    = σ₁.account_map ∧
    σ₀.hash_collision = σ₁.hash_collision ∧
    σ₀.execution_env  = σ₁.execution_env ∧
    σ₀.keccak_map     ≤ σ₁.keccak_map) := by
-  unfold preserved
-  dsimp
+  ext
+  apply Iff.intro
+  intro h
+  obtain ⟨_,_,_,_⟩ := h
+  all_goals tauto
 
-def preserved_account_map {evm evm' : EVMState} (h : preserved evm evm') :
-  evm.account_map = evm'.account_map := by
-  rw [preserved_def] at h
-  exact h.1
-
-def preserved_collision {evm evm' : EVMState} (h : preserved evm evm') :
-  evm.hash_collision = evm'.hash_collision := by
-  rw [preserved_def] at h
-  exact h.2.1
-
-def preserved_execution_env {evm evm' : EVMState} (h : preserved evm evm') :
-  evm.execution_env = evm'.execution_env := by
-  rw [preserved_def] at h
-  exact h.2.2.1
-
-def mono_keccak_map {evm evm' : EVMState} (h : preserved evm evm') :
-  evm.keccak_map ≤ evm'.keccak_map := by
-  rw [preserved_def] at h
-  exact h.2.2.2
+namespace Preserved
 
 @[simp]
-lemma preserved_rfl {e : EVM} : preserved e e := by
-  rw [preserved_def]
-  simp
+lemma refl {e : EVM} : Preserved e e := by
+  constructor
+  all_goals simp
 
-lemma preserved_trans {e₀ e₁ e₂ : EVM} :
-  preserved e₀ e₁ → preserved e₁ e₂ → preserved e₀ e₂ := by
-  rw (config := {occs := .pos [3]}) [preserved_def]
+lemma trans {e₀ e₁ e₂ : EVM} :
+  Preserved e₀ e₁ → Preserved e₁ e₂ → Preserved e₀ e₂ := by
   intro h₀ h₁
-  have acc := Eq.trans (preserved_account_map h₀) (preserved_account_map h₁)
-  have col := Eq.trans (preserved_collision h₀) (preserved_collision h₁)
-  have env := Eq.trans (preserved_execution_env h₀) (preserved_execution_env h₁)
-  have kec := le_trans (mono_keccak_map h₀) (mono_keccak_map h₁)
-  aesop
+  have acc := Eq.trans h₀.account_map h₁.account_map
+  have col := Eq.trans h₀.hash_collision h₁.hash_collision
+  have env := Eq.trans h₀.execution_env h₁.execution_env
+  have kec := le_trans h₀.keccak_map h₁.keccak_map
+  constructor <;> assumption
+
+end Preserved
+
+instance instPreorderEVMState : Preorder EVMState where
+  le := Preserved
+  le_refl := @Preserved.refl
+  le_trans := @Preserved.trans
 
 -- functions for querying balance
 
@@ -394,16 +385,16 @@ def evm_return (σ : EVMState) (mstart s : UInt256) : EVMState :=
 def evm_revert (σ : EVMState) (mstart s : UInt256) : EVMState :=
   σ.evm_return mstart s
 
-lemma mstore_preserved {σ} {pos val} : preserved σ (σ.mstore pos val) := by
+lemma mstore_preserved {σ} {pos val} : Preserved σ (σ.mstore pos val) := by
   unfold mstore updateMemory
-  rw [preserved_def]
+  rw [Preserved_def]
   simp
 
-lemma sload_eq_of_preserved {σ₀ σ₁} {pos} (h : preserved σ₀ σ₁) :
+lemma sload_eq_of_preserved {σ₀ σ₁} {pos} (h : Preserved σ₀ σ₁) :
   sload σ₀ pos = sload σ₁ pos := by
   unfold sload lookupAccount
-  rw [ preserved_account_map h
-     , preserved_execution_env h
+  rw [ h.account_map
+     , h.execution_env
      ]
 
 end
